---
title: "Lab 7: linear regression"
---

```{r setup, include=FALSE}
knitr::opts_chunk$set(echo = TRUE, message=FALSE)
```

## [Assignment link](https://goo.gl/forms/b2zXpiU6BGYo4zZe2)

```{r}
library(tidyverse)
library(GGally)
```

### 1.1
```{r}
df <- read.csv("http://goo.gl/Qo3Yy2")

df %>%
  ggplot(aes(mother, child))+
  geom_point()+
  geom_smooth(method = "lm", se = FALSE)

df %>%
  ggplot(aes(mother, child))+
  geom_point()+
  geom_smooth(method = "lm")+
  geom_point(aes(mean(mother), mean(child)), color = "tomato", size = 5)

cor(df)

fit <- lm(child~mother, data = df)
summary(fit)
ggplot(data = fit, aes(fit$fitted.values, fit$residuals))+
  geom_point()+
  geom_line(aes(y = 0))+
  labs(title = "fitted values ~ residuals",
       x = "fitted values",
       y = "residuals")

ggplot(data = fit, aes(sample = fit$residuals))+
  geom_qq()+
  labs(title = "qqplot for residuals")


predict(fit, data.frame(mother = 11:17/10))
```

### 2.
```{r}
df <- read.csv("https://goo.gl/TcyiRc", sep = "\t")

df %>% 
  ggplot(aes(r.frequency,rus.freq.dict))+
  geom_point(alpha = 0.2)+
  labs(titles = "relative frequencies from the short story and frequency dictionary",
       x = "relative frequencies from the short story",
       y = "relative frequencies from the frequency dictionary")

library(scales)
df %>% 
  ggplot(aes(r.frequency,rus.freq.dict))+
  geom_point(alpha = 0.2)+
    labs(titles = "relative frequencies from the short story and frequency dictionary",
         subtitle = "scales are with log transformation",
       x = "relative frequencies from the short story",
       y = "relative frequencies from the frequency dictionary")+
  scale_x_log10(labels = comma)+
  scale_y_log10(labels = comma)
```

### Remark on R formula syntax

* `y~x` gives you $y_i=\beta_0+\beta_1\times x_i$
* `y~x+z` gives you $y_i=\beta_0+\beta_1\times x_i+\beta_2\times z_i$
* `y~.` gives you $y_i=\beta_0+\beta_1\times x_i \dots \beta_k\times z_i$ (it makes a regression from all $k$ predictors)
* `y~1` gives you $y_i=\beta_0$
* `y~x-1` gives you $y_i=\beta_1\times x_i$
* `y~I(x-1)` gives you $y_i=\beta_0+\beta_1\times (x_i-1)$
* `y~I(x^2)` gives you $y_i=\beta_0+\beta_1\times x_i^2$